\documentclass[11pt]{article}
\usepackage{amssymb}
\usepackage{fullpage}
\usepackage{amsthm} 
\usepackage{changepage}
\pagestyle{empty}
\setlength{\parindent}{0pt}
\setlength{\parskip}{0.3cm}
\setlength{\parindent}{0cm}
%%% Sets
\newcommand{\nats}{\mathbb{N}}
\newcommand{\ints}{\mathbb{Z}}
\newcommand{\reals}{\mathbb{R}}
%%% Logic
\newcommand{\nnot}{\mathrm{NOT}}
\newcommand{\aand}{\,\,\mathrm{AND}\,\,}
\newcommand{\oor}{\,\,\mathrm{OR}\,\,}
\newcommand{\iimplies}{\,\,\mathrm{IMPLIES}\,\,}
\newcommand{\xor}{\,\,\mathrm{XOR}\,\,}
\newcommand{\iif}{\,\,\mathrm{IFF}\,\,}

\begin{document}

\begin{center}
{\Large CSC 240 Winter 2024 Quiz 4}
\end{center}

Give a well-structured informal proof by induction that,
for all natural numbers $n$ and for all integers $m \geq 2$,
$$
\sum_{k=0}^n m^k = \frac{m^{n+1}-1}{m-1}.
$$


\begin{proof}[Proof by induction]\hfill

    Let $P(n)="\displaystyle\sum_{k=0}^n m^k=\frac{m^{n+1}-1}{m-1}"$.

    Consider the base case where $n=0$. Then, we can see $\displaystyle\sum_{k=0}^n m^k=m^n=\sum_{k=0}^0 m^k=m^0=1=\frac{m^{0+1}-1}{m-1}=\frac{m^{n+1}-1}{m-1}$, this shows $P(0)$ holds;

    \begin{adjustwidth}{0.5cm}{}
        Now, pick an arbitrary $n\in\nats$;

        \begin{adjustwidth}{1cm}{}
            Assume $P(n)$ holds, i.e., $\displaystyle\sum_{k=0}^n m^k=\frac{m^{n+1}-1}{m-1}$;

            Then, we can see $\displaystyle\sum_{k=0}^{n+1} m^k=\displaystyle\sum_{k=0}^n m^k+m^{n+1}=\frac{m^{n+1}-1}{m-1}+m^{n+1}=\frac{m^{n+1}-1+m^{n+1}(m-1)}{m-1}=\frac{m^{n+1}-1+m^{n+2}-m^{n+1}}{m-1}=\frac{m^{n+2}-1}{m-1}=\frac{m^{(n+1)+1}-1}{m-1}$, we can see $P(n+1)$ also holds;
        \end{adjustwidth}
    \end{adjustwidth}

    By induction, we can conclude that $P(n)$ holds for all $n\in\nats$, this completes the proof.
\end{proof}

\end{document}
